---
title: "SMekala_Assign14"
author: "Sekhar Mekala"
date: "Sunday, November 15, 2015"
output: html_document
---

##Problem-1

Given that $$f(x) = \frac{1}{1-x}, \mbox{where }x \in (-1,1)$$

Let us expand this using Taylor series.
Let $a$ be a value between $(-1,1)$
$$f'(x) = \frac{1}{(1-x)^2} ==> f'(a) = \frac{1}{(1-a)^2}$$
$$f''(x) = \frac{2}{(1-x)^3} ==> f'(a) = \frac{2}{(1-a)^3}$$
$$f'''(x) = \frac{6}{(1-x)^4} ==> f'(a) = \frac{6}{(1-a)^4}$$
$$f''''(x) = \frac{24}{(1-x)^5} ==> f'(a) = \frac{24}{(1-a)^5}$$

Using Taylor series, we can say,

$$f(x) = \frac{1}{(1-x)} = f(a) + f'(a) (x-a) + f''(a) \frac{(x-a)^2}{2!} + f'''(a) \frac{(x-a)^3}{3!} + f''''(a) \frac{(x-a)^4}{4!} +...$$
$$ ==> \frac{1}{(1-x)} = \frac{1}{1-a} + \frac{1.(x-a)}{(1-a)^2} + \frac{2 . (x-a)^2}{(1-a)^3 . 2!} + \frac{6. (x-a)^3}{(1-a)^4 . 3!} + \frac{24 . (x-a)^4}{(1-a)^5 . 4!} +...$$
$$ ==> \frac{1}{(1-x)} = \frac{1}{1-a} + \frac{(x-a)}{(1-a)^2} + \frac{(x-a)^2}{(1-a)^3} + \frac{(x-a)^3}{(1-a)^4} + ... $$

Let us assume $a = 0$. Then the above expansion will become the Maclaurin Series.

$$ \frac{1}{(1-x)} = 1 + x + x^2 + x^3 + x^4 + ... $$
Hence, 
$$ \frac{1}{(1-x)} = 1 + x + x^2 + x^3 + x^4 + ... = \sum_{n=0}^{\infty} x^n, \mbox{where } x \in (-1,1)$$


##Problem-2

Given that $$f(x) = e^x,\mbox{where } x\in \mathbb{R}$$.

Let us expand this using Taylor series, at some value $x = a$.

$$f'(x) = e^x ==> f'(a) = e^a$$
$$f''(x) = e^x ==> f''(a) = e^a$$
$$f'''(x) = e^x ==> f'''(a) = e^a$$
$$f''''(x) = e^x ==> f''''(a) = e^a$$

Using Tayolr series, we can write the following:

$$f(x) = e^x = f'(a) (x - a) + f''(a) \frac{(x - a)^2}{2!} + f'''(a) \frac{(x-a)^3}{3!} + f''''(a) \frac{(x-a)^4}{4!} + +... $$
$$==> e^x = e^a + e^a (x - a) + e^a \frac{(x - a)^2}{2!} + e^a \frac{(x - a)^3}{3!} + e^a \frac{(x - a)^4}{4!} + ... $$

Let $a = 0$, then the above series will become Maclurin Series:

$$==> e^x = 1 +  x +  \frac{x^2}{2!} +  \frac{x^3}{3!} + \frac{x^4}{4!} + ... $$
Therefore,
$$==> e^x = 1 +  x +  \frac{x^2}{2!} +  \frac{x^3}{3!} + \frac{x^4}{4!} + ... = \sum_{n=0}^{\infty} \frac{x^n}{n!}, \mbox{where }x\in \mathbb{R}$$


##Problem-3

Given that $$f(x) = ln(1+x), \mbox{where }x\in (-1,1]$$.

Let us expand this using Taylor series, at some value $x = a, \mbox{where }a \in (-1,1]$.

$$f'(x) = \frac{1}{(1+x)} ==> f'(a) = \frac{1}{1+a}$$
$$f''(x) = \frac{-1}{(1+x)^2} ==> f'(a) = \frac{-1}{(1+a)^2}$$
$$f'''(x) = \frac{2}{(1+x)^3} ==> f'(a) = \frac{2}{(1+a)^3}$$
$$f''''(x) = \frac{-6}{(1+x)^4} ==> f'(a) = \frac{-6}{(1+a)^4}$$

Therefore,
$$f(x) = ln(1+x) = f(a) + f'(a) (x-a) +f''(a) \frac{(x-a)^2}{2!} + f'''(a) \frac{(x-a)^3}{3!} + f''''(a) \frac{(x-a)^4}{4!} + ...$$
$$==> ln(1+x) = ln(1 + a) + \frac{1}{(1+a)} (x-a) - \frac{1}{(1+a)^2 . 2!} (x-a)^2 +  \frac{2}{(1+a)^3 . 3!} (x-a)^3 - \frac{6}{(1+a)^4 . 4!} (x-a)^4 + ...$$

$$==> ln(1+x) = ln(1 + a) + \frac{1}{(1+a)} (x-a) - \frac{1}{(1+a)^2 . 2} (x-a)^2 +  \frac{1}{(1+a)^3 . 3} (x-a)^3 - \frac{1}{(1+a)^4 . 4} (x-a)^4 + ...$$

Let us assume $a = 0$, then the above series will become Maclaurin series, give the following expansion:

$$==> ln(1+x) = ln(1) + x - \frac{x^2}{2} +  \frac{x^3}{3} - \frac{x^4}{4} + ...$$
$$==> ln(1+x) = x - \frac{x^2}{2} +  \frac{x^3}{3} - \frac{x^4}{4} + ...$$
$$==> ln(1+x) = \sum_{n=1}^{\infty}(-1)^{n+1} \frac{x^n}{n}, \mbox{where }x\in (-1,1]$$


                                                     ~~~**End of Assignment**~~